Updating Handling of Local + Global contexts.

S4/S4.v
@@ -18,7 +18,7 @@ Inductive ty : Type :=
 
 Inductive tm : Type :=
 (* Pure STLC terms*)
-| tm_var    : string -> tm
+| local_var : string -> tm
 | tm_app    : tm -> tm -> tm
 | tm_abs    : string -> ty -> tm -> tm
 (* Booleans *)
@@ -26,6 +26,7 @@ Inductive tm : Type :=
 | tm_false  : tm
 | tm_if     : tm -> tm -> tm -> tm
 (* Box operators *)
+| global_var : string -> tm
 | tm_box    : tm -> tm
 | tm_unbox  : string -> tm -> tm -> tm
 (* Diamond operators *)
@@ -48,7 +49,6 @@ Notation "\ x : t , y" :=
                      t custom stlc_ty at level 99,
                      y custom stlc_tm at level 99,
                      left associativity).
-Coercion tm_var : string >-> tm.
 
 (* Notations for boolean expressions + types *)
 Notation "'Bool'" := Ty_Bool (in custom stlc_ty at level 0).
@@ -84,15 +84,24 @@ Open Scope string_scope.
 (** Some more notation magic to set up the concrete syntax, as we did
     in the [Imp] chapter... *)
 
-Definition x : string := "x".
-Definition y : string := "y".
-Definition z : string := "z".
-Definition u : string := "u".
-Definition w : string := "w".
-Definition t : string := "t".
-Definition f : string := "f".
-Definition g : string := "g".
-Definition s : string := "s".
+Definition LocalVar := string.
+Definition  LiftLocalVar : LocalVar -> tm := local_var.
+Coercion  LiftLocalVar : LocalVar >-> tm.
+
+Definition GlobalVar := string.
+Definition LiftGlobalVar : GlobalVar -> tm := global_var.
+Coercion  LiftGlobalVar : GlobalVar >-> tm.
+
+Definition x : LocalVar := "x".
+Definition y : LocalVar := "y".
+Definition z : LocalVar := "z".
+Definition f : LocalVar := "f".
+Definition g : LocalVar := "g".
+
+Definition u : GlobalVar := "u".
+Definition w : GlobalVar := "w".
+Definition t : GlobalVar := "t".
+Definition s : GlobalVar := "s".
 
 Hint Unfold x : core.
 Hint Unfold y : core.
@@ -110,7 +119,7 @@ Definition quote A : tm := <{\x : □ A, unbox u := x in box (box u) }>.
    : □(Bool ⊃ Bool) ⊃ □Bool ⊃ □A *)
 Definition apply A B : tm := <{\x : □ (A -> B), \y : □ A,
           unbox u := x in
-        unbox w := y in box (u w) }>.
+          unbox w := y in box (u w) }>.
 
 (* A proof of ♢♢Bool -> ♢Bool *)
 (* λx: ♢♢ Bool. dia (let dia y = x in let dia z = y in z)*)
@@ -164,7 +173,7 @@ Reserved Notation "'[' x ':=' s ']' t" (in custom stlc_tm at level 20, x constr)
 
 Fixpoint local_subst (x : string) (s : tm) (t : tm) : tm :=
   match t with
-  | tm_var y =>
+  | local_var y =>
       if x =? y then s else t
   | <{\y : T , t1}> =>
       if x =? y then t else <{\y : T, [x:=s] t1}>
@@ -179,52 +188,51 @@ Fixpoint local_subst (x : string) (s : tm) (t : tm) : tm :=
       <{if ([x:=s] t1) then ([x:=s] t2) else ([x:=s] t3)}>
 
   (* Box operators *)
+  | global_var u => global_var u
   | <{ box t }> =>
       <{ box t }>
   | <{ unbox y := t1 in t2 }> =>
-      if x =? y then <{ unbox y := [x := s] t1 in t2 }>
-      else <{ unbox y := [x := s] t1 in [x := s] t2 }>
+      <{ unbox y := [x := s] t1 in [x := s] t2 }>
   (* Diamond operators *)
   | <{ dia t }> =>
       <{ dia ([x := s] t) }>
   | <{ undia y := t1 in t2 }> =>
-      if x =? y then <{ undia y := [x := s] t1 in t2 }>
-      else <{ undia y := [x := s] t1 in [x := s] t2 }>
+      (*if x =? y then  *)
+       <{ undia y := [x := s] t1 in t2 }>
+      (*else <{ undia y := [x := s] t1 in [x := s] t2 }> *)
   end
 
 where "'[' x ':=' s ']' t" := (local_subst x s t) (in custom stlc_tm).
 
-
 Reserved Notation "'[[' x ':=' s ']]' t" (in custom stlc_tm at level 20, x constr).
 
-Fixpoint global_subst (x : string) (s : tm) (t : tm) : tm :=
+Fixpoint global_subst (u : string) (s : tm) (t : tm) : tm :=
   match t with
-  | tm_var y =>
-      if x =? y then s else t
-  | <{\y : T , t1}> =>
-      if x =? y then t else <{\y : T, [[x:=s]] t1}>
+  | local_var y => local_var y
+  | <{\y : T , t1}> => <{\y : T, [[u:=s]] t1}>
   | <{t1 t2}> =>
-    <{([[x:=s]] t1) ([[x:=s]] t2)}>
+    <{([[u:=s]] t1) ([[u:=s]] t2)}>
   (* Booleans *)
   | <{ true }>  =>
       <{ true }>
   | <{ false }> =>
       <{ false }>
   | <{if t1 then t2 else t3}> =>
-      <{if ([[x:=s]] t1) then ([[x:=s]] t2) else ([[x:=s]] t3)}>
+      <{if ([[u:=s]] t1) then ([[u:=s]] t2) else ([[u:=s]] t3)}>
 
   (* Box operators *)
+  | global_var v =>
+      if u =? v then s else t
   | <{ box t }> =>
-      <{ box [[x:=s]] t }>
+      <{ box [[u:=s]] t }>
   | <{ unbox y := t1 in t2 }> =>
-      if x =? y then <{ unbox y := [[x := s]] t1 in t2 }>
-      else <{ unbox y := [[x := s]] t1 in [[x := s]] t2 }>
+      if u =? y then <{ unbox y := [[u := s]] t1 in t2 }>
+      else <{ unbox y := [[u := s]] t1 in [[u := s]] t2 }>
   (* Diamond operators *)
   | <{ dia t }> =>
-      <{ dia ([[x := s]] t) }>
+      <{ dia ([[u := s]] t) }>
   | <{ undia y := t1 in t2 }> =>
-      if x =? y then <{ undia y := [[x := s]] t1 in t2 }>
-      else <{ undia y := [[x := s]] t1 in [[x := s]] t2 }>
+      <{ undia y := [[u := s]] t1 in [[u := s]] t2 }>
   end
 
 where "'[[' x ':=' s ']]' t" := (global_subst x s t) (in custom stlc_tm).
@@ -340,88 +348,67 @@ Ltac normalize_lambda :=
   repeat (eapply multi_step;
           [ simpl; next_step | simpl ]).
 
-Reserved Notation "Gamma '|-' t '\in' T"
+Reserved Notation "Delta ';;' Gamma '|-' t '\in' T"
             (at level 101,
              t custom stlc_tm, T custom stlc_ty at level 0).
 
-Inductive var_scope :=
-| local : ty -> var_scope
-| global : ty -> var_scope.
+Definition context := partial_map ty.
 
-Definition context := partial_map var_scope.
-
-Definition global_context (Gamma : context) : context :=
-  fun x => match Gamma x with
-           | Some (global T) => Some (global T)
-           | _ => None
-           end.
-
-Lemma global_context_OK :
-  forall Gamma,
-    ((forall x T, Gamma x = Some (global T) -> (global_context Gamma) x = Some (global T)) /\
-       (forall x T, (global_context Gamma) x = Some (global T) -> Gamma x = Some (global T)) /\
-       (forall x T, (global_context Gamma) x <> Some (local T))).
-Proof.
-  unfold global_context; intuition; try rewrite H; eauto.
-  destruct (Gamma x0) as [ [? | ?] | ]; simpl in *; congruence.
-  destruct (Gamma x0) as [ [? | ?] | ]; simpl in *; congruence.
-Qed.
-
-Inductive has_type : context -> tm -> ty -> Prop :=
+Inductive has_type : context -> context -> tm -> ty -> Prop :=
 (* Lambda Terms *)
-| T_Var1 : forall Gamma x T1,
-    Gamma x = Some (local T1) ->
-    Gamma |- x \in T1
-| T_Var2 : forall Gamma x T1,
-    Gamma x = Some (global T1) ->
-    Gamma |- x \in T1
-| T_Abs : forall Gamma x T1 T2 t1,
-    x |-> local T2 ; Gamma |- t1 \in T1 ->
-      Gamma |- \x:T2, t1 \in (T2 -> T1)
-| T_App : forall T1 T2 Gamma t1 t2,
-      Gamma |- t1 \in (T2 -> T1) ->
-      Gamma |- t2 \in T2 ->
-      Gamma |- t1 t2 \in T1
+| T_Local_Var : forall Delta Gamma x T1,
+    Gamma x = Some T1 ->
+    has_type Delta Gamma (local_var x) T1
+| T_Abs : forall Delta Gamma x T1 T2 t1,
+    Delta;;  x |-> T2 ; Gamma |- t1 \in T1 ->
+    Delta;; Gamma |- \x:T2, t1 \in (T2 -> T1)
+| T_App : forall Delta Gamma T1 T2 t1 t2,
+      Delta;; Gamma |- t1 \in (T2 -> T1) ->
+      Delta;; Gamma |- t2 \in T2 ->
+      Delta;; Gamma |- t1 t2 \in T1
 
 (* Booleans *)
-| T_True : forall Gamma,
-      Gamma |- true \in Bool
-| T_False : forall Gamma,
-       Gamma |- false \in Bool
-| T_If : forall t1 t2 t3 T1 Gamma,
-    Gamma |- t1 \in Bool ->
-    Gamma |- t2 \in T1 ->
-       Gamma |- t3 \in T1 ->
-       Gamma |- if t1 then t2 else t3 \in T1
+| T_True : forall Delta Gamma,
+      Delta ;; Gamma |- true \in Bool
+| T_False : forall Delta Gamma,
+       Delta;; Gamma |- false \in Bool
+| T_If : forall Delta Gamma t1 t2 t3 T1,
+    Delta;; Gamma |- t1 \in Bool ->
+    Delta;; Gamma |- t2 \in T1 ->
+       Delta;; Gamma |- t3 \in T1 ->
+       Delta;; Gamma |- if t1 then t2 else t3 \in T1
 
 (* Box Operators *)
-| T_Box : forall Gamma t T,
-    global_context Gamma |- t \in T ->
-    Gamma |- box t \in □T
-| T_Unbox : forall Gamma x t1 t2 T1 T2 ,
-    Gamma |- t1 \in ( □T1 ) ->
-    (x |-> global T1; Gamma) |- t2 \in T2  ->
-    Gamma |- unbox x := t1 in t2 \in T2
+| T_Global_Var : forall Delta Gamma u T1,
+    Delta u = Some T1 ->
+    has_type Delta Gamma (global_var u) T1
+| T_Box : forall Delta Gamma t T,
+    Delta;; empty  |- t \in T ->
+    Delta;; Gamma |- box t \in □T
+| T_Unbox : forall Delta Gamma x t1 t2 T1 T2 ,
+    Delta;; Gamma |- t1 \in ( □T1 ) ->
+    (x |-> T1; Delta) ;; Gamma |- t2 \in T2  ->
+    Delta;; Gamma |- unbox x := t1 in t2 \in T2
 
 (* Dia Operators *)
-| T_Dia : forall Gamma t T,
-    has_local_type Gamma t T ->
-    Gamma |- dia t \in ♢T
+| T_Dia : forall Delta Gamma t T,
+    has_local_type Delta Gamma t T ->
+    Delta;; Gamma |- dia t \in ♢T
 
-with has_local_type : context -> tm -> ty -> Prop :=
-| LT_Undia : forall Gamma x t1 t2 T1 T2 ,
-    Gamma |- t1 \in ( ♢T1 ) ->
-    has_local_type (x |-> local T1; global_context Gamma) t2 T2  ->
-    has_local_type Gamma <{undia x := t1 in t2}> T2
-| LT_Unbox : forall Gamma x t1 t2 T1 T2 ,
-    Gamma |- t1 \in ( □T1 ) ->
-    has_local_type (x |-> global T1; Gamma) t2 T2  ->
-    has_local_type Gamma <{unbox x := t1 in t2}> T2
-| LT_global : forall Gamma t T,
-    Gamma |- t \in T ->
-    has_local_type Gamma t T
+with has_local_type : context -> context -> tm -> ty -> Prop :=
+| LT_Undia : forall Delta Gamma x t1 t2 T1 T2 ,
+    Delta;; Gamma |- t1 \in ( ♢T1 ) ->
+    has_local_type Delta (x |-> T1; empty) t2 T2  ->
+    has_local_type Delta Gamma <{undia x := t1 in t2}> T2
+| LT_Unbox : forall Delta Gamma x t1 t2 T1 T2 ,
+    Delta;; Gamma |- t1 \in ( □T1 ) ->
+    has_local_type (x |-> T1; Delta) Gamma t2 T2  ->
+    has_local_type Delta Gamma <{unbox x := t1 in t2}> T2
+| LT_global : forall Delta Gamma t T,
+    Delta;; Gamma |- t \in T ->
+    has_local_type Delta Gamma t T
 
-where "Gamma '|-' t '\in' T" := (has_type Gamma t T).
+where "Delta ';;' Gamma '|-' t '\in' T" := (has_type Delta Gamma t T).
 
 Scheme has_type_ind' := Induction for has_type Sort Prop
   with has_local_type_ind' := Induction for has_local_type Sort Prop.
@@ -431,7 +418,7 @@ Scheme has_type_ind' := Induction for has_type Sort Prop
 (* λx:A ⊃ B ⊃ C. λy:A ⊃ B. λz:A. (x z) (y z)
    : (A ⊃ B ⊃ C) ⊃(A ⊃ B) ⊃ A ⊃ C *)
 Example Modal_Axiom_1 : forall A B C,
-   empty |- \x:A -> B -> C, \y:A -> B, \z:A, (x z) (y z)
+   empty;; empty |- \x:A -> B -> C, \y:A -> B, \z:A, (x z) (y z)
    \in ((A -> B -> C) -> (A -> B) -> A -> C).
 Proof.
   repeat econstructor.
@@ -440,7 +427,7 @@ Qed.
 (* λx:A. λy:B. x
    : A ⊃ B ⊃ A *)
 Example Modal_Axiom_2 : forall A B,
-    empty |- \x : A, \y : B, x \in (A -> B -> A).
+    empty;; empty |- \x : A, \y : B, x \in (A -> B -> A).
 Proof.
   repeat econstructor.
 Qed.
@@ -448,50 +435,33 @@ Qed.
 (* λx:□(A ⊃ B). λy:□A. let box u = x in let box w = y in box (u w)
    : □(A ⊃ B) ⊃(□A ⊃ □B) *)
 Example Modal_Axiom_3 : forall A B,
-    empty |-
+    empty;; empty |-
       \x:□(A -> B), \y:□A, (unbox u := x in unbox w := y in box (u w))
         \in ((□(A -> B)) -> (□A) -> (□B)).
 Proof.
-  intros; econstructor.
-  econstructor.
-  econstructor.
-  - repeat econstructor.
-  - econstructor.
-    + repeat econstructor.
-    + econstructor.
-      econstructor.
-      constructor 2; reflexivity.
-      constructor 2; reflexivity.
+  intros; repeat econstructor.
 Qed.
 
 (* λx:□A. let box u = x in u
 : □A ⊃ A *)
 Example Modal_Axiom_4 : forall A,
-    empty |- \y : □A, unbox u := y in u \in ((□A) -> A).
+    empty;; empty |- \y : □A, unbox u := y in u \in ((□A) -> A).
 Proof.
-  econstructor.
-  econstructor.
   repeat econstructor.
-  econstructor 2; reflexivity.
 Qed.
 
 (* λx:□A. let box u = x in box box u
    : □A ⊃ □□A *)
 Example Modal_Axiom_5 : forall A,
-    empty |- \x : □A, unbox u := x in box (box u) \in ((□A) -> (□ (□ A))).
+    empty;; empty |- \x : □A, unbox u := x in box (box u) \in ((□A) -> (□ (□ A))).
 Proof.
-  econstructor.
-  econstructor.
   repeat econstructor.
-  econstructor.
-  econstructor.
-  econstructor 2; reflexivity.
 Qed.
 
 (* λx:A. dia x
    : A ⊃ ♢A *)
 Example Modal_Axiom_6 : forall A,
-    empty |- \x : A, dia x \in (A -> ♢A).
+    empty;; empty |- \x : A, dia x \in (A -> ♢A).
 Proof.
   repeat econstructor.
 Qed.
@@ -499,7 +469,7 @@ Qed.
 (* λx:♢♢A. dia (let dia y = x in let dia z = y in z)
    : ♢♢A ⊃ ♢A *)
 Example Modal_Axiom_7 : forall A,
-    empty |- \x : ♢♢A, dia (undia y := x in undia z := y in z) \in ((♢♢A) -> ♢A).
+    empty;; empty |- \x : ♢♢A, dia (undia y := x in undia z := y in z) \in ((♢♢A) -> ♢A).
 Proof.
   repeat econstructor.
 Qed.
@@ -507,72 +477,43 @@ Qed.
 (* λx:□(A ⊃ B). λy:♢A. let box u = x in dia (let dia z = y in u z)
    : □(A ⊃ B) ⊃(♢A ⊃ ♢B) *)
 Example Modal_Axiom_8 : forall A B,
-    empty |- \x : □(A -> B), \y : ♢A, unbox u := x in dia (undia z := y in u z)
+    empty;; empty |- \x : □(A -> B), \y : ♢A, unbox u := x in dia (undia z := y in u z)
                                                                    \in ((□(A -> B)) -> (♢A) -> ♢B).
 Proof.
-  econstructor.
-  econstructor.
-  econstructor.
-  - repeat econstructor.
-  - econstructor.
-    econstructor.
-    + repeat econstructor.
-    + econstructor.
-      econstructor.
-      * econstructor 2; reflexivity.
-      * repeat econstructor.
+  repeat econstructor.
 Qed.
 
 (* λx: A ⊃ B. λy:♢A. let box u = x in dia (let dia z = y in u z)
    : (A ⊃ B) ⊃(♢A ⊃ ♢B) *)
 Example Modal_Axiom_8' : forall A B,
-    ~ (empty |- \x : A -> B, \y : ♢A, dia (undia z := y in x z) \in (((A -> B)) -> (♢A) -> ♢B)).
+    ~ (empty;; empty |- \x : A -> B, \y : ♢A, dia (undia z := y in x z) \in (((A -> B)) -> (♢A) -> ♢B)).
 Proof.
   unfold not; intros.
-  inversion H; subst; clear H.
-  inversion H2; subst; clear H2.
-  inversion H1; subst; clear H1.
-  inversion H3; subst; clear H3.
-  - inversion H6; subst; clear H6.
-    inversion H; subst; clear H.
-    inversion H3; subst; clear H3.
-    compute in H1; discriminate.
-    compute in H1; discriminate.
-  - inversion H.
+  repeat match goal with
+           H : _ ;; _ |- _ \in _ |- _ => inversion H; subst; clear H
+         | H : has_local_type _ _ _  _ |- _ => inversion H; subst; clear H
+         end.
+    compute in H3; discriminate.
 Qed.
 
 Example quote_is_typed (A : ty) :
   let t := quote A in
-  empty |- t \in ((□A) -> (□□A)).
+  empty;; empty |- t \in ((□A) -> (□□A)).
 Proof.
-  econstructor.
-  econstructor.
-  - repeat econstructor.
-  - econstructor.
-    econstructor.
-    econstructor 2; reflexivity.
+  repeat econstructor.
 Qed.
 
 Example apply_is_typed (A B : ty) :
   let t := apply A B in
-  empty |- t \in ((□A -> B) -> (□A) -> □B).
+  empty;; empty |- t \in ((□A -> B) -> (□A) -> □B).
 Proof.
-  econstructor.
-  econstructor.
-  econstructor.
-  - repeat econstructor.
-  - econstructor.
-    + repeat econstructor.
-    + econstructor.
-      econstructor.
-      econstructor 2; reflexivity.
-      econstructor 2; reflexivity.
+  repeat econstructor.
 Qed.
 
 Hint Constructors has_type.
 
 Lemma canonical_forms_bool : forall t,
-  empty |- t \in Bool ->
+  empty;; empty |- t \in Bool ->
   value t ->
   (t = <{true}>) \/ (t = <{false}>).
 Proof.
@@ -581,7 +522,7 @@ Proof.
 Qed.
 
 Lemma canonical_forms_fun : forall t T1 T2,
-  empty |- t \in (T1 -> T2) ->
+    empty;; empty |- t \in (T1 -> T2) ->
   value t ->
   exists x u, t = <{\x:T1, u}>.
 Proof.
@@ -590,7 +531,7 @@ Proof.
 Qed.
 
 Lemma canonical_forms_box : forall t T,
-  empty |- t \in (□ T) ->
+  empty;; empty |- t \in (□ T) ->
   value t ->
   exists u, t = <{box u}>.
 Proof.
@@ -599,7 +540,7 @@ Proof.
 Qed.
 
 Lemma canonical_forms_diamond : forall t T,
-  empty |- t \in (♢ T) ->
+  empty;; empty |- t \in (♢ T) ->
   value t ->
   exists u, t = <{dia u}>.
 Proof.
@@ -608,11 +549,14 @@ Proof.
 Qed.
 
 Theorem progress : forall t T,
-  empty |- t \in T ->
+  empty;; empty |- t \in T ->
   value t \/ exists t', t --> t'.
 Proof with eauto.
   intros t T Ht.
   remember empty as Gamma.
+  rewrite HeqGamma in Ht at 1.
+  remember empty as Delta.
+  rewrite HeqDelta in HeqGamma.
   induction Ht; try injection HeqGamma; intros; subst;
     try discriminate; try solve [left; constructor].
   - (* T_App *)
@@ -634,7 +578,6 @@ Proof with eauto.
       econstructor; eauto.
   - (* T_If *)
     right. destruct IHHt1...
-
     + (* t1 is a value *)
       destruct (canonical_forms_bool t1); subst; eauto.
       * exists t2; econstructor; eauto.
@@ -651,568 +594,186 @@ Proof with eauto.
       eexists; econstructor; eauto.
 Qed.
 
-Lemma inclusion_global_context :
-  forall Gamma Gamma',
+Lemma inclusion_trans :
+  forall Gamma Gamma' Gamma'' : context,
     inclusion Gamma Gamma' ->
-    inclusion (global_context Gamma) (global_context Gamma').
+    inclusion Gamma' Gamma'' ->
+    inclusion Gamma Gamma''.
 Proof.
-  unfold global_context, inclusion; intros.
-  destruct (Gamma x0) eqn: ?.
-  - erewrite H; eauto.
-  - discriminate.
+  unfold inclusion; intros; eauto.
 Qed.
 
-Lemma inclusion_global_context_local_update :
-  forall x T T' Gamma,
-    inclusion (x |-> T; (global_context (x |-> T'; Gamma))) (x |-> T; global_context Gamma).
+Lemma inclusion_refl :
+  forall Gamma : context,
+    inclusion Gamma Gamma.
 Proof.
-  unfold global_context, inclusion; intros.
-  unfold update, t_update in *.
-  destruct (eqb_string x0 x1) eqn: ?; try discriminate; congruence.
+  unfold inclusion; intros; eauto.
 Qed.
 
-Lemma weakening : forall Gamma Gamma' t T,
+Lemma weakening : forall Delta Delta' Gamma Gamma' t T,
+    inclusion Delta Delta' ->
     inclusion Gamma Gamma' ->
-    Gamma  |- t \in T  -> Gamma' |- t \in T.
+    Delta;; Gamma  |- t \in T  -> Delta';; Gamma' |- t \in T.
 Proof.
-  intros Gamma Gamma' t T HInc Ht;
-    revert Gamma' HInc.
-  pattern Gamma, t, T, Ht;
+  intros Delta Delta' Gamma Gamma' t T HIncD HIncG Ht;
+    revert Delta' Gamma' HIncD HIncG.
+  pattern Delta, Gamma, t, T, Ht;
     eapply has_type_ind' with
-    (P := fun Gamma t T _ => forall Gamma' : partial_map var_scope, inclusion Gamma Gamma' -> Gamma' |- t \in T)
-    (P0 := fun Gamma t T _ => forall Gamma' : partial_map var_scope, inclusion Gamma Gamma' -> has_local_type Gamma' t T); eauto using inclusion_update; clear; intros.
+    (P := fun Delta Gamma t T _ => forall Delta' Gamma' : context,
+              inclusion Delta Delta' ->
+              inclusion Gamma Gamma' ->
+              Delta';; Gamma' |- t \in T)
+    (P0 := fun Delta Gamma t T _ => forall Delta' Gamma' : context,
+               inclusion Delta Delta' ->
+               inclusion Gamma Gamma' ->
+               has_local_type Delta' Gamma' t T); eauto using inclusion_update; clear; intros.
   - econstructor.
     eapply H; eauto; compute; eauto.
-    unfold inclusion in H0.
-    intros; specialize (H0 x0 v); destruct (Gamma x0) as [ [? | ?] | ]; try congruence.
-    rewrite H0; injection H1; intros; subst; congruence.
   - econstructor; eauto.
-    eapply H0; eauto using inclusion_update, inclusion_global_context.
+    eapply H0; eauto using inclusion_update, inclusion_refl.
   - econstructor; eauto using inclusion_update.
   - econstructor; eauto.
 Qed.
 
-Lemma local_weakening : forall Gamma Gamma' t T,
+Lemma local_weakening : forall Delta Delta' Gamma Gamma' t T,
+    inclusion Delta Delta' ->
     inclusion Gamma Gamma' ->
-    has_local_type Gamma t T  -> has_local_type Gamma' t T.
+    has_local_type Delta Gamma t T  ->
+    has_local_type Delta' Gamma' t T.
 Proof.
-  intros Gamma Gamma' t T HInc Ht;
-    revert Gamma' HInc;
+  intros Delta Delta' Gamma Gamma' t T HIncD HIncG Ht;
+    revert Delta' Gamma' HIncD HIncG;
     induction Ht; simpl; intros;
-    econstructor; eauto using weakening, inclusion_update, inclusion_global_context.
+    econstructor; eauto using weakening, inclusion_update, inclusion_refl.
 Qed.
 
 Lemma local_substitution_preserves_typing
-  : forall Gamma x U t v T,
-  (x |-> local U; Gamma) |- t \in T ->
-  empty |- v \in U   ->
-  Gamma |- [x:=v]t \in T.
+  : forall Delta Gamma x U t v T,
+    Delta;; (x |-> U; Gamma) |- t \in T ->
+  empty;; empty |- v \in U   ->
+  Delta;; Gamma |- [x:=v]t \in T.
 Proof.
-  intros Gamma x U t v T Ht.
-  remember (x |-> local U; Gamma) as Gamma'.
-  assert (inclusion Gamma'  (x |-> local U; Gamma)) by
-    (rewrite HeqGamma'; unfold inclusion; congruence).
-  clear HeqGamma'.
+  intros Delta Gamma x U t v T Ht.
+  remember (x |-> U; Gamma) as Gamma'.
   generalize dependent Gamma.
-  pattern Gamma', t, T, Ht;
+  revert x U.
+  pattern Delta, Gamma', t, T, Ht;
     eapply has_type_ind' with
-    (P := fun Gamma' t T _ =>
-            forall
-              (Gamma : partial_map var_scope)
-              (Heq : inclusion Gamma' (x |-> local U; Gamma))
-              (Hv : empty |- v \in U),
-              Gamma |- [x := v] t \in T)
-    (P0 := fun Gamma' t T _ =>
-             forall
-               (Gamma : partial_map var_scope)
-               (Heq : inclusion Gamma' (x |-> local U; Gamma))
-               (Hv : empty |- v \in U),
-               has_local_type Gamma (<{[x := v] t}>) T);
+    (P := fun Delta Gamma' t T _ =>
+            forall x U
+              (Gamma : context)
+              (Heq : Gamma' = (x |-> U; Gamma))
+              (Hv : empty;; empty |- v \in U),
+              Delta;; Gamma |- [x := v] t \in T)
+    (P0 := fun Delta Gamma' t T _ =>
+             forall x U
+               (Gamma : context)
+               (Heq : Gamma' = (x |-> U; Gamma))
+               (Hv : empty;; empty |- v \in U),
+               has_local_type Delta Gamma (<{[x := v] t}>) T);
     eauto using inclusion_update; clear; intros; subst; simpl; eauto.
   - (* var1 *)
-    rename x0 into y. destruct (eqb_stringP x y); subst.
+    rename x0 into y.
+    rename x1 into x.
+    destruct (eqb_stringP x y); subst.
     + (* x=y *)
-      eapply Heq in e; rewrite update_eq in e.
+      rewrite update_eq in e.
       injection e as H2; subst.
       rewrite eqb_refl; intros; eapply weakening; try eassumption;
-        unfold inclusion; eauto.
-      compute; congruence.
+        unfold inclusion; eauto;
+        compute; congruence.
     + (* x<>y *)
-      apply Heq in e.
       rewrite (proj2 (eqb_neq x y)); eauto.
-      intros; apply T_Var1.
+      intros; apply T_Local_Var.
       rewrite update_neq in e; auto.
-  - rename x0 into y. destruct (eqb_stringP x y); eapply Heq in e; subst.
-    + (* x=y *)
-      rewrite update_eq in e; congruence.
-    + (* x<>y *)
-      rewrite (proj2 (eqb_neq x y)); eauto.
-      intros; apply T_Var2. rewrite update_neq in e; auto.
   - (* abs *)
+    rename x1 into x.
     rename x0 into y.
     destruct (eqb_stringP x y); subst.
     + (* x=y *)
-      rewrite eqb_refl.
-      apply T_Abs.
-      eapply weakening; try eassumption.
-      admit.
-      (*rewrite update_shadow in h. assumption. *)
+      rewrite eqb_refl; rewrite update_shadow in h; eauto.
     +  (* x<>y *)
       rewrite (proj2 (eqb_neq x y)); eauto.
       apply T_Abs.
-      apply H; eauto.
-      rewrite update_permute; auto using inclusion_update.
-  - (* box *)
-    econstructor.
-    eapply weakening; try eassumption.
-    admit.
-    (*unfold inclusion; simpl; intros.
-    unfold update, t_update, global_context in *|-*.
-    destruct (eqb_stringP x x0); subst; eauto.
-    congruence. *)
+      eapply H; eauto.
+      rewrite update_permute; auto.
+  - (* undia *)
+    econstructor; eauto.
   - rename x0 into y.
-    destruct (eqb_stringP x y); subst.
-    + (* x=y *)
-      rewrite eqb_refl.
-      admit.
-      (*rewrite update_shadow in h0.
-      econstructor; eauto. *)
-    +  (* x<>y *)
-      rewrite (proj2 (eqb_neq x y)); eauto.
-      eapply T_Unbox.
-      * apply H; eauto.
-      * eapply H0; eauto.
-        rewrite update_permute; auto using inclusion_update.
-  - rename x0 into y.
-    destruct (eqb_stringP x y); subst.
-    + (* x=y *)
-      rewrite eqb_refl.
-      econstructor; eauto.
-      admit.
-      (*eapply local_weakening; eauto using inclusion_update, inclusion_global_context_local_update. *)
-    +  (* x<>y *)
-      rewrite (proj2 (eqb_neq x y)); eauto.
-      eapply LT_Undia.
-      * apply H; eauto.
-      * eapply H0; eauto.
-        rewrite update_permute by congruence.
-        eapply inclusion_update.
-        apply inclusion_global_context in Heq.
-        admit.
-  - rename x0 into y.
-    destruct (eqb_stringP x y); subst.
-    + (* x=y *)
-      rewrite eqb_refl.
-      admit.
-    +  (* x<>y *)
-      rewrite (proj2 (eqb_neq x y)); eauto.
-      eapply LT_Unbox.
-      * apply H; eauto.
-      * eapply H0; eauto.
-        rewrite update_permute; auto.
-        admit.
+    eapply LT_Unbox.
+    + eapply H; eauto.
+    + eapply H0; eauto.
   - econstructor; eauto.
-Admitted.
-
-Inductive bound_in : string -> tm -> Prop :=
-  | bi_app1 : forall x t1 t2,
-      bound_in x t1 -> bound_in x <{ t1 t2 }>
-  | bi_app2 : forall x t1 t2,
-      bound_in x t2 -> bound_in x <{ t1 t2 }>
-| bi_abs : forall x T11 t12,
-    bound_in x <{ \x : T11, t12 }>
-| bi_abs2 : forall x y T11 t12,
-    bound_in x <{ t12 }> ->
-    bound_in x <{ \y : T11, t12 }>
-
-  (* booleans *)
-  | bi_test0 : forall x t0 t1 t2,
-      bound_in x t0 ->
-      bound_in x <{ if t0 then t1 else t2 }>
-  | bi_test1 : forall x t0 t1 t2,
-      bound_in x t1 ->
-      bound_in x <{ if t0 then t1 else t2 }>
-  | bi_test2 : forall x t0 t1 t2,
-      bound_in x t2 ->
-      bound_in x <{ if t0 then t1 else t2 }>
-  (* Modal Operators  *)
-  | bi_box : forall x t1,
-      bound_in x t1 ->
-      bound_in x <{ box t1 }>
-| bi_unbox1 : forall x t1 t2,
-    bound_in x <{ unbox x := t1 in t2 }>
-| bi_unbox2 : forall x y t1 t2,
-      bound_in x t1 ->
-      bound_in x <{ unbox y := t1 in t2 }>
-| bi_unbox3 : forall x y t1 t2,
-    bound_in x t2 ->
-    bound_in x <{ unbox y := t1 in t2 }>
-
-| bi_dia : forall x t1,
-      bound_in x t1 ->
-      bound_in x <{ dia t1 }>
-| bi_undia1 : forall x t1 t2,
-      bound_in x <{ undia x := t1 in t2 }>
-| bi_undia2 : forall x y t1 t2,
-      bound_in x t1 ->
-      bound_in x <{ undia y := t1 in t2 }>
-| bi_undia3 : forall x y t1 t2,
-    bound_in x t2 ->
-    bound_in x <{ undia y := t1 in t2 }>.
-
-Hint Constructors bound_in : core.
-
-Inductive appears_free_in : string -> tm -> Prop :=
-  | afi_var : forall (x : string),
-      appears_free_in x <{ x }>
-  | afi_app1 : forall x t1 t2,
-      appears_free_in x t1 -> appears_free_in x <{ t1 t2 }>
-  | afi_app2 : forall x t1 t2,
-      appears_free_in x t2 -> appears_free_in x <{ t1 t2 }>
-  | afi_abs : forall x y T11 t12,
-        y <> x  ->
-        appears_free_in x t12 ->
-        appears_free_in x <{ \y : T11, t12 }>
-
-  (* booleans *)
-  | afi_test0 : forall x t0 t1 t2,
-      appears_free_in x t0 ->
-      appears_free_in x <{ if t0 then t1 else t2 }>
-  | afi_test1 : forall x t0 t1 t2,
-      appears_free_in x t1 ->
-      appears_free_in x <{ if t0 then t1 else t2 }>
-  | afi_test2 : forall x t0 t1 t2,
-      appears_free_in x t2 ->
-      appears_free_in x <{ if t0 then t1 else t2 }>
-  (* Modal Operators  *)
-  | afi_box : forall x t1,
-      appears_free_in x t1 ->
-      appears_free_in x <{ box t1 }>
-| afi_unbox1 : forall x y t1 t2,
-    appears_free_in x t2 ->
-    appears_free_in x <{ unbox y := t1 in t2 }>
-| afi_unbox2 : forall x y t1 t2,
-    x <> y ->
-    appears_free_in x t2 ->
-    appears_free_in x <{ unbox y := t1 in t2 }>
-| afi_dia : forall x t1,
-      appears_free_in x t1 ->
-      appears_free_in x <{ dia t1 }>
-  | afi_undia1 : forall x y t1 t2,
-      appears_free_in x t2 ->
-      appears_free_in x <{ undia y := t1 in t2 }>
-| afi_undia2 : forall x y t1 t2,
-    x <> y ->
-    appears_free_in x t2 ->
-    appears_free_in x <{ undia y := t1 in t2 }>.
-
-Hint Constructors appears_free_in : core.
-
-Lemma inclusion_update_empty
-  : forall x T (Gamma : context),
-    inclusion (x |-> T) (x |-> T; Gamma).
-Proof.
-  unfold inclusion, update, t_update;
-    intros; destruct (eqb_stringP x0 x1); subst; eauto.
-  discriminate.
 Qed.
 
-Lemma local_substitution_preserves_typing'
-  : forall Gamma Gamma'' x U t v T
-           (Hx : forall x, bound_in x t -> Gamma'' x = None)
-           (HInc : inclusion Gamma'' Gamma),
-  (x |-> local U; Gamma) |- t \in T ->
-  Gamma'' |- v \in U   ->
-  Gamma |- [x:=v]t \in T.
+Theorem local_substitution_preserves_local_typing
+  : forall Delta Gamma x U t v T,
+    has_local_type Delta (x |-> U; Gamma) t T ->
+    empty;; empty |- v \in U   ->
+  has_local_type Delta Gamma <{[x:=v]t}> T.
 Proof.
-  intros Gamma Gamma'' x U t v T Hx HInc Ht.
-  remember (x |-> local U; Gamma) as Gamma'.
-  revert Hx HInc.
-  generalize dependent Gamma.
-  revert Gamma''.
-  pattern Gamma', t, T, Ht;
-    eapply has_type_ind' with
-    (P := fun Gamma' t T _ =>
-            forall
-              (Gamma'' Gamma : partial_map var_scope)
-              (Heq : Gamma' = (x |-> local U; Gamma))
-              (Hx : forall x, bound_in x t -> Gamma'' x = None)
-              (HInc : inclusion Gamma'' Gamma)
-              (Hv : Gamma'' |- v \in U),
-              Gamma |- [x := v] t \in T)
-    (P0 := fun Gamma' t T _ =>
-             forall
-               (Gamma'' Gamma : partial_map var_scope)
-               (Heq : Gamma' = (x |-> local U; Gamma))
-               (Hx : forall x, bound_in x t -> Gamma'' x = None)
-               (HInc : inclusion Gamma'' Gamma)
-               (Hv : Gamma'' |- v \in U),
-               has_local_type Gamma (<{[x := v] t}>) T);
-    eauto using inclusion_update; clear; intros; subst; simpl; eauto.
-  - (* var1 *)
-    rename x0 into y. destruct (eqb_stringP x y); subst.
-    + (* x=y *)
-      rewrite update_eq in e.
-      injection e as H2; subst.
-      rewrite eqb_refl; intros; eapply weakening; try eassumption;
-        unfold inclusion; eauto.
-    + (* x<>y *)
-      rewrite (proj2 (eqb_neq x y)); eauto.
-      intros; apply T_Var1. rewrite update_neq in e; auto.
-  - rename x0 into y. destruct (eqb_stringP x y); subst.
-    + (* x=y *)
-      rewrite update_eq in e; congruence.
-    + (* x<>y *)
-      rewrite (proj2 (eqb_neq x y)); eauto.
-      intros; apply T_Var2. rewrite update_neq in e; auto.
-  - (* abs *)
-    rename x0 into y.
-    destruct (eqb_stringP x y); subst.
-    + (* x=y *)
-      rewrite eqb_refl.
-      apply T_Abs.
-      rewrite update_shadow in h. assumption.
-    +  (* x<>y *)
-      rewrite (proj2 (eqb_neq x y)); eauto.
-      apply T_Abs.
-      eapply H with (Gamma'' := Gamma''); eauto.
-      rewrite update_permute; auto.
-      * unfold inclusion, update, t_update.
-        intros; destruct (eqb_stringP y x0); subst; eauto.
-        rewrite Hx in H0; try discriminate; eauto.
-  - econstructor; eauto.
-  - econstructor; eauto.
-  - (* box *)
-    econstructor.
-    eapply weakening; try eassumption.
-    unfold inclusion; simpl; intros.
-    unfold update, t_update, global_context in *|-*.
-    destruct (eqb_stringP x x0); subst; eauto.
-    congruence.
-  - rename x0 into y.
-    destruct (eqb_stringP x y); subst.
-    + (* x=y *)
-      rewrite eqb_refl.
-      rewrite update_shadow in h0.
-      econstructor; eauto.
-    +  (* x<>y *)
-      rewrite (proj2 (eqb_neq x y)); eauto.
-      eapply T_Unbox.
-      * eapply H; eauto.
-      * eapply H0; eauto.
-        rewrite update_permute; auto.
-        unfold inclusion; simpl; intros.
-        unfold update, t_update, global_context.
-        destruct (eqb_stringP y x0); subst; eauto.
-        rewrite Hx in H1; eauto; try discriminate.
-  - rename x0 into y.
-    destruct (eqb_stringP x y); subst.
-    + (* x=y *)
-      rewrite eqb_refl.
-      econstructor; eauto using local_weakening, inclusion_update, inclusion_global_context_local_update.
-    +  (* x<>y *)
-      rewrite (proj2 (eqb_neq x y)); eauto.
-      admit.
-      (* eapply LT_Undia. *)
-      (* * eapply H; eauto. *)
-      (* * eapply H0; eauto. *)
-      (*   rewrite update_permute; auto. *)
-      (*   unfold inclusion, update, t_update, global_context; intros. *)
-      (*   destruct (eqb_stringP y x0); subst; eauto. *)
-      (*   rewrite Hx in H1; eauto; try discriminate. *)
-  - rename x0 into y.
-    destruct (eqb_stringP x y); subst.
-    + (* x=y *)
-      rewrite eqb_refl.
-      rewrite update_shadow in h0.
-      econstructor; eauto.
-    +  (* x<>y *)
-      rewrite (proj2 (eqb_neq x y)); eauto.
-      eapply LT_Unbox.
-      * eapply H; eauto.
-      * eapply H0; eauto.
-        rewrite update_permute; auto.
-        unfold inclusion, update, t_update, global_context; intros.
-        destruct (eqb_stringP y x0); subst; eauto.
-        rewrite Hx in H1; eauto; try discriminate.
-  - econstructor; eauto.
-Admitted.
-
-Lemma local_substitution_preserves_local_typing'
-  : forall Gamma Gamma'' x U t v T
-           (Hx : forall x, bound_in x t -> Gamma'' x = None)
-           (HInc : inclusion Gamma'' Gamma),
-    has_local_type (x |-> local U; Gamma) t  T ->
-    Gamma'' |- v \in U ->
-    has_local_type Gamma <{[x:=v]t}> T.
-Proof.
-  intros Gamma Gamma'' x U t v T Hx HInc Ht.
-  remember (x |-> local U; Gamma) as Gamma'.
-  generalize dependent Gamma.
-  induction Ht; intros; simpl.
-  - rename x0 into y.
-    destruct (eqb_stringP x y); subst.
-    + (* x=y *)
-      rewrite eqb_refl.
-      econstructor; eauto using local_substitution_preserves_typing'.
-      eapply local_weakening; eauto using inclusion_global_context_local_update,
-        inclusion_update.
-    +  (* x<>y *)
-      rewrite (proj2 (eqb_neq x y)); eauto.
-      eapply LT_Undia; eauto using local_substitution_preserves_typing'.
-      admit.
-      (* eapply IHHt; eauto using local_substitution_preserves_typing'.
-      * unfold inclusion, update, t_update, global_context; intros.
-        destruct (eqb_stringP y x0); subst; eauto.
-        rewrite Hx in H1; eauto; try discriminate.
-      * rewrite update_permute; auto. *)
-  - rename x0 into y.
-    destruct (eqb_stringP x y); subst.
-    + (* x=y *)
-      rewrite eqb_refl.
-      rewrite update_shadow in Ht.
-      econstructor; eauto using local_substitution_preserves_typing'.
-    +  (* x<>y *)
-      rewrite (proj2 (eqb_neq x y)); eauto.
-      eapply LT_Unbox; eauto using local_substitution_preserves_typing'.
-      eapply IHHt; eauto using local_substitution_preserves_typing'.
-      * unfold inclusion, update, t_update, global_context; intros.
-        destruct (eqb_stringP y x0); subst; eauto.
-        rewrite Hx in H1; eauto; try discriminate.
-      * rewrite update_permute; auto.
-  - subst; econstructor; eauto using local_substitution_preserves_typing'.
-Admitted.
-
-(*Theorem local_substitution_preserves_local_typing : forall Gamma x U t v T,
-    has_local_type (x |-> local U; Gamma) t T ->
-    empty |- v \in U   ->
-  has_local_type Gamma <{[x:=v]t}> T.
-Proof.
-  intros Gamma x U t v T Ht.
-  remember (x |-> local U; Gamma) as Gamma'.
+  intros Delta Gamma x U t v T Ht.
+  remember (x |-> U; Gamma) as Gamma'.
   generalize dependent Gamma.
   induction Ht; intros; subst; simpl; eauto.
-  - rename x0 into y.
-    destruct (eqb_stringP x y); subst.
-    + (* x=y *)
-      rewrite eqb_refl.
-      rewrite update_shadow in Ht.
-      econstructor; eauto.
-      eapply local_substitution_preserves_typing; try eassumption.
-    +  (* x<>y *)
-      rewrite (proj2 (eqb_neq x y)); eauto.
-      econstructor.
-      * eapply local_substitution_preserves_typing;
-          try eassumption; try reflexivity; discriminate.
-      * eapply IHHt; eauto.
-        rewrite update_permute; auto.
-  - rename x0 into y.
-    destruct (eqb_stringP x y); subst.
-    + (* x=y *)
-      rewrite eqb_refl.
-      rewrite update_shadow in Ht.
-      econstructor; eauto.
-      eapply local_substitution_preserves_typing;
-        try eassumption; try reflexivity; discriminate.
-    + rewrite (proj2 (eqb_neq x y)); eauto.
-      econstructor; eauto using local_substitution_preserves_typing;
+  - econstructor; eauto.
+    eapply local_substitution_preserves_typing;
+      try eassumption; try reflexivity; discriminate.
+  - econstructor; eauto using local_substitution_preserves_typing;
         try eassumption; try reflexivity; try discriminate.
-      eapply IHHt; eauto.
-      rewrite update_permute; auto.
   - econstructor; eauto using local_substitution_preserves_typing.
-Qed. *)
+Qed.
 
-Lemma global_substitution_preserves_typing : forall Gamma x U t v T,
-  (x |-> global U; Gamma) |- t \in T ->
-  empty |- v \in U   ->
-  Gamma |- [[x:=v]]t \in T.
+Lemma global_substitution_preserves_typing : forall Delta Gamma x U t v T,
+  (x |-> U; Delta);; Gamma |- t \in T ->
+  empty;; empty |- v \in U   ->
+  Delta;; Gamma |- [[x:=v]]t \in T.
 Proof.
-  intros Gamma x U t v T Ht.
-  remember (x |-> global U; Gamma) as Gamma'.
-  generalize dependent Gamma.
-  pattern Gamma', t, T, Ht;
+  intros Delta Gamma x U t v T Ht.
+  remember (x |-> U; Delta) as Delta'.
+  generalize dependent Delta.
+  pattern Delta', Gamma, t, T, Ht;
     eapply has_type_ind' with
-    (P := fun Gamma' t T _ =>
+    (P := fun Delta' Gamma t T _ =>
             forall
-              (Gamma : partial_map var_scope)
-              (Heq : Gamma' = (x |-> global U; Gamma))
-                   (Hv : empty |- v \in U),
-              Gamma |- [[x := v]] t \in T)
-    (P0 := fun Gamma' t T _ =>
+              (Delta : context)
+              (Heq : Delta' = (x |-> U; Delta))
+              (Hv : empty;; empty |- v \in U),
+              Delta;; Gamma |- [[x := v]] t \in T)
+    (P0 := fun Delta' Gamma t T _ =>
              forall
-               (HId : has_local_type Gamma' t T)
-               (Gamma : partial_map var_scope)
-                    (Heq : Gamma' = (x |-> global U; Gamma))
-                    (Hv : empty |- v \in U),
-               has_local_type Gamma (<{[[x := v]] t}>) T);
+               (HId : has_local_type Delta' Gamma t T)
+               (Delta : context)
+               (Heq : Delta' = (x |-> U; Delta))
+               (Hv : empty;; empty |- v \in U),
+               has_local_type Delta Gamma (<{[[x := v]] t}>) T);
     eauto using inclusion_update; clear; intros; subst; simpl; eauto.
-  - (* var1 *)
-    rename x0 into y. destruct (eqb_stringP x y); subst.
+  - (* global_var *)
+    rename u0 into u. destruct (eqb_stringP x u); subst.
     + (* x=y *)
       rewrite update_eq in e.
       injection e as H2; subst.
       rewrite eqb_refl; intros; eapply weakening; try eassumption;
-        unfold inclusion; eauto.
-      compute; discriminate.
+        unfold inclusion; eauto;
+        compute; discriminate.
     + (* x<>y *)
-      rewrite (proj2 (eqb_neq x y)); eauto.
-      intros; apply T_Var1. rewrite update_neq in e; auto.
-  - rename x0 into y. destruct (eqb_stringP x y); subst.
-    + (* x=y *)
-      rewrite eqb_refl.
-      rewrite update_eq in e; injection e; intros; subst.
-      eapply weakening; eauto.
-      compute; congruence.
-    + (* x<>y *)
-      rewrite (proj2 (eqb_neq x y)); eauto.
-      intros; apply T_Var2. rewrite update_neq in e; auto.
-  - (* abs *)
-    rename x0 into y.
-    destruct (eqb_stringP x y); subst.
-    + (* x=y *)
-      rewrite eqb_refl.
-      apply T_Abs.
-      rewrite update_shadow in h. assumption.
-    +  (* x<>y *)
-      rewrite (proj2 (eqb_neq x y)); eauto.
-      apply T_Abs.
-      apply H; eauto.
-      rewrite update_permute; auto.
-  - (* box *)
-    econstructor.
-    eapply H; eauto.
-    eapply functional_extensionality; intros.
-    unfold update, t_update, global_context in *|-*.
-    destruct (eqb_stringP x x0); subst; eauto.
-  - rename x0 into y.
-    destruct (eqb_stringP x y); subst.
+      rewrite (proj2 (eqb_neq x u)); eauto.
+      intros; apply T_Global_Var. rewrite update_neq in e; auto.
+  - (* unbox *)
+    rename x0 into y. destruct (eqb_stringP x y); subst.
     + (* x=y *)
       rewrite eqb_refl.
       rewrite update_shadow in h0.
       econstructor; eauto.
-    +  (* x<>y *)
+    + (* x<>y *)
       rewrite (proj2 (eqb_neq x y)); eauto.
-      eapply T_Unbox.
-      * apply H; eauto.
-      * eapply H0; eauto.
-        rewrite update_permute; auto.
-  - rename x0 into y.
-    destruct (eqb_stringP x y); subst.
-    + (* x=y *)
-      rewrite eqb_refl.
       econstructor; eauto.
-      eapply local_weakening; eauto using inclusion_global_context_local_update,
-        inclusion_update.
-    +  (* x<>y *)
-      rewrite (proj2 (eqb_neq x y)); eauto.
-      eapply LT_Undia.
-      * apply H; eauto.
-      * eapply H0; eauto.
-        rewrite update_permute by congruence.
-        f_equal.
-        apply functional_extensionality; intros.
-        unfold global_context, update, t_update.
-        destruct (eqb_string x x0) eqn: ?; eauto.
+      eapply H0; eauto.
+      rewrite update_permute; eauto.
+  - rename x0 into y.
+    eapply LT_Undia.
+    + apply H; eauto.
+    + eapply H0; eauto.
   - rename x0 into y.
     destruct (eqb_stringP x y); subst.
     + (* x=y *)
@@ -1228,30 +789,17 @@ Proof.
   - econstructor; eauto.
 Qed.
 
-Theorem global_substitution_preserves_local_typing : forall Gamma x U t v T,
-    has_local_type (x |-> global U; Gamma) t T ->
-  empty |- v \in U   ->
-  has_local_type Gamma <{[[x:=v]]t}> T.
+Theorem global_substitution_preserves_local_typing
+  : forall Delta Gamma x U t v T,
+    has_local_type (x |-> U; Delta) Gamma t T ->
+  empty;; empty |- v \in U   ->
+  has_local_type Delta Gamma <{[[x:=v]]t}> T.
 Proof.
-  intros Gamma x U t v T Ht.
-  remember (x |-> global U; Gamma) as Gamma'.
-  generalize dependent Gamma.
+  intros Delta Gamma x U t v T Ht.
+  remember (x |-> U; Delta) as Delta'.
+  generalize dependent Delta.
   induction Ht; intros; subst; simpl; eauto.
-  - rename x0 into y.
-    destruct (eqb_stringP x y); subst.
-    + (* x=y *)
-      rewrite eqb_refl.
-      econstructor; eauto using global_substitution_preserves_typing.
-      eapply local_weakening; eauto using inclusion_global_context_local_update.
-    +  (* x<>y *)
-      rewrite (proj2 (eqb_neq x y)); eauto.
-      econstructor; eauto using global_substitution_preserves_typing.
-      eapply IHHt; eauto.
-      rewrite update_permute; auto.
-      f_equal.
-      apply functional_extensionality; intros.
-      unfold global_context, update, t_update.
-      destruct (eqb_string x x0) eqn: ?; eauto.
+  - econstructor; eauto using global_substitution_preserves_typing.
   - rename x0 into y.
     destruct (eqb_stringP x y); subst.
     + (* x=y *)
@@ -1265,138 +813,81 @@ Proof.
   - econstructor; eauto using global_substitution_preserves_typing.
 Qed.
 
-Definition disjoint_contexts (Gamma Gamma' : context) : Prop :=
-  (forall x T, Gamma x = Some T -> Gamma' x = None) /\
-    (forall x T, Gamma' x = Some T -> Gamma x = None).
-
-Definition union_contexts (Gamma Gamma' : context) : context :=
-  fun x => match Gamma x with
-           | Some T => Some T
-           | _ => Gamma' x
-           end.
-
-Lemma union_empty : forall (Gamma : context),
-    union_contexts Gamma empty = Gamma.
-Proof.
-  intros; apply functional_extensionality.
-  intros; unfold union_contexts; destruct (Gamma x0); eauto.
-Qed.
-
-Lemma disjoint_empty : forall (Gamma : context),
-    disjoint_contexts Gamma empty.
-Proof.
-  unfold disjoint_contexts; split; simpl; intros.
-  reflexivity.
-  discriminate.
-Qed.
-
-Lemma inclusion_union : forall (Gamma Gamma' : context),
-    inclusion Gamma (union_contexts Gamma Gamma').
-Proof.
-  unfold inclusion, union_contexts; intros.
-  destruct (Gamma x0); congruence.
-Qed.
-
-Lemma lookup_disjoint_contexts
-      : forall (Gamma Gamma' : context),
-      disjoint_contexts Gamma Gamma' ->
-      forall x T, Gamma' x = Some T ->
-                  (union_contexts Gamma Gamma') x = Some T.
-Proof.
-  unfold union_contexts; intros.
-  unfold disjoint_contexts in H; intuition.
-  specialize (H1 x0).
-  destruct (Gamma x0); eauto.
-  erewrite H1 in H0; try discriminate; reflexivity.
-Qed.
-
-Lemma inclusion_union_2 : forall (Gamma Gamma' : context),
-    disjoint_contexts Gamma Gamma' ->
-    inclusion Gamma' (union_contexts Gamma Gamma').
-Proof.
-  unfold inclusion; intros.
-  eauto using lookup_disjoint_contexts.
-Qed.
-
-Lemma local_substitution_preserves_local_typing''
-  : forall Gamma Gamma'' x U t v T
-           (Hx : forall x, bound_in x t -> ~ bound_in x v)
-           (HInc : disjoint_contexts Gamma'' Gamma),
-    has_local_type (x |-> local U; Gamma) t  T ->
-    Gamma'' |- v \in U ->
-    has_local_type (union_contexts Gamma'' Gamma) <{[x:=v]t}> T.
-Proof.
-Admitted.
-
 Lemma delaying_preserves_local_typing
-  : forall Gamma x U t v T
-           (NIn_x : Gamma x = None)
-           (NIn_x_2 : ~ bound_in x v)
-           (Hx : forall x, bound_in x t -> ~ bound_in x v),
-    has_local_type (x |-> local U) t T ->
-    has_local_type Gamma v U   ->
-    has_local_type Gamma <{〈 x := v〉t}> T.
+  : forall x U t v T,
+    has_local_type empty (x |-> U) t T ->
+    has_local_type empty empty v U   ->
+    has_local_type empty empty <{〈 x := v〉t}> T.
 Proof.
-  intros Gamma x U t v T NIn_x NIn_x2 Hx Ht He.
-  revert NIn_x2 NIn_x Hx.
+  intros x U t v T Ht Hv.
+  remember empty as Gamma.
+  rewrite HeqGamma in Hv at 1, Ht at 1.
+  rewrite HeqGamma at 1.
+  remember empty as Delta.
+  rewrite HeqDelta in HeqGamma.
   generalize dependent T.
-  pattern Gamma, v, U, He.
+  revert HeqDelta HeqGamma.
+  pattern Delta, Gamma, v, U, Hv.
     eapply has_local_type_ind' with
-      (P := (fun (o : context) (t0 : tm) (t1 : ty) (_ : has_type o t0 t1) =>
-               forall (T : ty),
-                 has_local_type (x |-> local t1) t T ->
-                 (~ bound_in x t0) ->
-                 (o x = None ) ->
-                 (forall x, bound_in x t -> ~ bound_in x t0) ->
-                 has_local_type o <{ 〈 x := t0〉  t }> T))
-      (P0 := (fun (o : context) (t0 : tm) (t1 : ty) (_ : has_local_type o t0 t1) =>
-               forall (T : ty),
-                 has_local_type (x |-> local t1) t T ->
-                 (~ bound_in x t0) ->
-                 (o x = None) ->
-                 (forall x, bound_in x t -> ~ bound_in x t0) ->
-                   has_local_type o <{ 〈 x := t0 〉 t }> T));
-      try solve [simpl; intros;
-                 rewrite <- (union_empty Gamma0);
-                 eapply local_substitution_preserves_local_typing'';
-                 unfold inclusion; eauto using local_weakening, inclusion_update_empty, disjoint_empty];
-      eauto.
-  - simpl; econstructor; eauto.
+      (P := (fun Delta Gamma v U _ =>
+               forall
+                 (HeqDelta : Delta = empty)
+                 (HeqGamma : Gamma = empty) (T : ty),
+                 has_local_type Delta (x |-> U; Gamma) t T ->
+                 has_local_type Delta Gamma <{ 〈 x := v〉  t }> T))
+      (P0 := (fun Delta Gamma v U _ =>
+                forall
+                 (HeqDelta : Delta = empty)
+                 (HeqGamma : Gamma = empty) (T : ty),
+                 has_local_type Delta (x |-> U; Gamma) t T ->
+                 has_local_type Delta Gamma <{ 〈 x := v〉  t }> T));
+      simpl; intros;
+      try solve [subst;
+                 eauto using local_substitution_preserves_local_typing].
+  - admit.
+    (* simpl; econstructor; eauto.
     eapply H0; eauto using inclusion_update.
     + unfold update, t_update; simpl.
       destruct (eqb_stringP x0 x); subst; eauto.
       destruct H2; eauto.
     + unfold not; intros.
-      eapply H4; eauto.
-  - simpl; econstructor; eauto.
+      eapply H4; eauto. *)
+  - admit.
+    (* simpl; econstructor; eauto.
     eapply H0; eauto using inclusion_update.
     + unfold update, t_update; simpl.
       destruct (eqb_stringP x0 x); subst; eauto.
       destruct H2; eauto.
       unfold global_context; rewrite H3; reflexivity.
     + unfold not; intros.
-      eapply H4; eauto.
+      eapply H4; eauto. *)
   - simpl; econstructor; eauto.
-    eapply H0; eauto using inclusion_update.
-    + unfold update, t_update; simpl.
-      destruct (eqb_stringP x0 x); subst; eauto.
-      destruct H2; eauto.
-    + unfold not; intros.
-      eapply H4; eauto.
-Qed.
+    admit.
+Admitted.
 
 (* Alas, it appears that we cannot escape variable renaming :p *)
 
 Theorem preservation : forall t t' T,
-  empty |- t \in T  ->
+  empty;; empty |- t \in T  ->
   t --> t'  ->
-  empty |- t' \in T.
+  empty;; empty |- t' \in T.
 Proof with eauto.
   intros t t' T HT. generalize dependent t'.
   remember empty as Gamma.
+  rewrite HeqGamma in HT at 1.
+  remember empty as Delta.
+  rewrite HeqDelta in HeqGamma.
+  setoid_rewrite HeqGamma at 1.
+  rewrite <- HeqDelta.
   eapply has_type_ind' with
-    (P := fun Gamma t T _ => Gamma = empty ->  forall (t' : tm) (HE : t --> t'), Gamma |- t' \in T)
-    (P0 := fun Gamma t T _ =>  Gamma = empty ->  forall (t' : tm) (HE : t --> t'), has_local_type Gamma t' T)
+    (P := fun Delta Gamma t T _ =>
+            Delta = empty ->
+            Gamma = empty ->
+            forall (t' : tm) (HE : t --> t'), Delta;; Gamma |- t' \in T)
+    (P0 := fun Delta Gamma t T _ =>
+             Delta = empty ->
+             Gamma = empty ->
+             forall (t' : tm) (HE : t --> t'), has_local_type Delta Gamma t' T)
     in HT; eauto; clear; intros; subst; try discriminate;
     try solve [inversion HE; subst; auto].
   - (* T_App *)
@@ -1410,12 +901,9 @@ Proof with eauto.
     + econstructor; eauto.
     + inversion h; subst.
       eapply delaying_preserves_local_typing; try eassumption.
-      reflexivity.
-      admit.
-      admit.
   - inversion HE; subst...
     + econstructor; eauto.
     + eapply global_substitution_preserves_local_typing; eauto.
       inversion h; subst; assumption.
   - econstructor; eauto.
-Admitted.
+Qed.
